src/arch/x64/X64.Semantics_Equiv_i.fsti
@@ -7,14 +7,32 @@ open X64.Semantics_s
 val equiv_eval_ins (s:state) (ins:S.ins) : Lemma (
    let s_hi = run (eval_ins ins) s in
    let s_bytes = S.run (S.eval_ins ins) s.state in
+   (s_hi.state.S.ok ==> s_bytes.S.ok) /\
    s_hi.state.S.ok /\ s_bytes.S.ok ==> s_hi.state == s_bytes)
 
-// val equiv_eval_code (s:state) (fuel:nat) (code:code) : Lemma (
-//   let s_hi = eval_code code fuel s in
-//   let s_bytes = S.eval_code code fuel s.state in
-//     (None? s_hi /\ None? s_bytes) \/
-//   ( Some? s_hi /\ Some? s_bytes /\ 
-//     ((Some?.v s_hi).state.S.ok /\ (Some?.v s_bytes).S.ok ==> 
-//     (Some?.v s_hi).state == Some?.v s_bytes
-//   ))
-// )
+val equiv_eval_code (code:code) (fuel:nat) (s:state) : Lemma 
+  (requires True)
+  (ensures 
+  (let s_hi = eval_code code fuel s in
+   let s_bytes = S.eval_code code fuel s.state in
+  Some? s_hi /\ Some? s_bytes /\ (Some?.v s_hi).state.S.ok /\ (Some?.v s_bytes).S.ok ==>
+  (Some?.v s_hi).state == Some?.v s_bytes))
+  (decreases %[fuel; code])
+
+val equiv_eval_codes (l:codes) (fuel:nat) (s:state) : Lemma 
+  (requires True)
+  (ensures 
+  (let s_hi = eval_codes l fuel s in
+  let s_bytes = S.eval_codes l fuel s.state in
+  Some? s_hi /\ Some? s_bytes /\ (Some?.v s_hi).state.S.ok /\ (Some?.v s_bytes).S.ok ==>
+  (Some?.v s_hi).state == Some?.v s_bytes))
+  (decreases %[fuel; l])
+
+val equiv_eval_while (b:ocmp) (c:code) (fuel:nat) (s:state) : Lemma 
+  (requires True)
+  (ensures (
+  let s_hi = eval_while b c fuel s in
+  let s_bytes = S.eval_while b c fuel s.state in
+  Some? s_hi /\ Some? s_bytes /\ (Some?.v s_hi).state.S.ok /\ (Some?.v s_bytes).S.ok ==>
+  (Some?.v s_hi).state == Some?.v s_bytes))
+  (decreases %[fuel; c])
